Added some theorems and proofs

LeanMathLogicExploration/RelationalAlgebra.lean
@@ -1,15 +1,12 @@
 import MathLib.Tactic
 set_option pp.coercions false
 
-#check Relation
-
-
 universe u v
 
-abbrev RelationPairs α β  := (a:α) -> (b:β) -> Prop
+abbrev Relation.Pairs α β  := (a:α) -> (b:β) -> Prop
 
-inductive Relation : (Dom Cod : Type u) -> Type (max u v + 1 )
-| atomic (f:RelationPairs α β) : Relation α β
+inductive Relation : (Dom Cod : Type u) -> Type (max u + 1 )
+| atomic (f:Relation.Pairs α β) : Relation α β
 | comp (R:Relation α β) (S:Relation β γ) : Relation α γ
 | full (α β: Type u): Relation α β
 | id  (α: Type u)  :  Relation α α
@@ -30,16 +27,17 @@ def Relation.par (R: Relation α β )(S: Relation γ δ) : Relation (α × γ ) 
 
 def Relation.with (R: Relation α β )(S: Relation γ δ) :=  neg (coproduct (neg R) (neg S))
 
-def Relation.same (α : Type u) := converse (copy α)
+def Relation.empty (α β :Type u) := complement (full α β)
 
-def Relation.different (α: Type u) := complement (equals α)
+def Relation.same (α : Type u) := converse (copy α)
+def Relation.different (α: Type u) := neg (copy α)
 
 def Relation.domain (_: Relation α β) := α
 def Relation.codomain (_: Relation α β) := β
 
 -- Relation.eval takes a relation and returns a function that tells use whether a pair is in the function.
-def Relation.eval (R:Relation α β) : RelationPairs α β :=
-match R with
+def Relation.eval (R':Relation α β) : Relation.Pairs α β :=
+match R' with
 | atomic f => f
 | comp R S => fun (a : R.domain) (b : S.codomain) =>
   ∃ (c : S.domain), Relation.eval R a c ∧ Relation.eval S c b
@@ -54,3 +52,191 @@ match R with
   | Sum.inr a', Sum.inr b' => Relation.eval S a' b'
   | _, _ => False
 | copy α => fun a (a1, a2) => a = a1 ∧ a = a2
+
+
+
+@[simp]
+theorem Relation.double_converse (R: Relation α β) : eval (converse (converse R)) = eval R := by
+  apply funext; intro a; apply funext; intro b
+  simp [Relation.eval, Relation.converse]
+
+@[simp]
+theorem Relation.double_complement (R: Relation α β) : eval (complement (complement R)) = eval R := by
+  apply funext; intro a; apply funext; intro b
+  simp [Relation.eval, Relation.complement]
+
+@[simp]
+theorem Relation.double_neg (R: Relation α β) : eval (neg (neg R)) = eval R := by
+  apply funext; intro a; apply funext; intro b
+  simp [Relation.eval, Relation.neg,  Relation.complement, Relation.converse]
+
+-- complement-converse equals converse-complement and we simply to the later.
+@[simp]
+theorem Relation.converse_complement_sym (R: Relation α β) : eval (complement (converse R)) =  eval (converse ( complement  R))  := by
+  apply funext; intro b; apply funext; intro a;
+  simp [Relation.eval]
+
+-- Complement-converse simplifies to negation
+@[simp]
+theorem Relation.complement_converse_to_neg (R: Relation α β) : eval (complement (converse R)) = eval (neg R) := by
+  apply funext; intro b; apply funext; intro a;
+  simp [Relation.eval, Relation.neg]
+
+
+-- Composition is associative
+theorem Relation.assoc_comp (R: Relation α β) (S: Relation β γ) (T: Relation γ δ) :
+  eval (comp (comp R S) T) = eval (comp R (comp S T)) := by
+  apply funext; intro a; apply funext; intro d
+  simp [Relation.eval, Relation.comp]
+  apply Iff.intro
+  . intro ⟨c, ⟨b, hab, hbc⟩, hcd⟩
+    exact ⟨b, hab, ⟨c, hbc, hcd⟩⟩
+  . intro ⟨b, hab, ⟨c, hbc, hcd⟩⟩
+    exact ⟨c, ⟨b, hab, hbc⟩, hcd⟩
+
+-- Converse distributes over composition
+@[simp]
+theorem Relation.converse_comp (R: Relation α β) (S: Relation β γ) :
+  eval (converse (comp R S)) = eval (comp (converse S) (converse R)) := by
+  apply funext; intro c; apply funext; intro a
+  simp [Relation.eval, Relation.comp, Relation.converse]
+  apply Iff.intro
+  . intro ⟨b, hab, hbc⟩
+    exact ⟨b, hbc, hab⟩
+  . intro ⟨b, hcb, hba⟩
+    exact ⟨b, hba, hcb⟩
+
+-- Complement distributes over composition?
+
+-- Negation distributes over composition?
+
+-- Converse distributes across product
+@[simp]
+theorem Relation.converse_product (R: Relation α β) (S: Relation γ δ) :
+  eval (converse (product R S)) = eval (product (converse R) (converse S)) := by
+  apply funext; intro ⟨b, d⟩; apply funext; intro ⟨a, c⟩
+  simp [Relation.eval, Relation.product, Relation.converse]
+
+-- Complement distributes across product
+@[simp]
+theorem Relation.complement_product (R: Relation α β) (S: Relation γ δ) :
+  eval (complement (product R S)) = eval (par (complement R) (complement S)) := by
+  apply funext; intro ⟨a, c⟩; apply funext; intro ⟨b, d⟩
+  simp [Relation.eval]
+
+@[simp]
+theorem Relation.neg_product (R: Relation α β) (S: Relation γ δ) :
+  eval (neg (product R S)) = eval (par (neg R) (neg S)) := by
+  apply funext; intro ⟨a, c⟩; apply funext; intro ⟨b, d⟩
+  simp [Relation.eval]
+
+@[simp]
+theorem Relation.converse_coproduct (R: Relation α β) (S: Relation γ δ) :
+  eval (converse (coproduct R S)) = eval (coproduct (converse R) (converse S)) := by
+  apply funext; intro ab; apply funext; intro cd
+  cases ab <;> cases cd
+  . simp [Relation.eval]
+  . simp [Relation.eval]
+  . simp [Relation.eval]
+  . simp [Relation.eval]
+
+@[simp]
+theorem Relation.complement_coproduct (R: Relation α β) (S: Relation γ δ) :
+eval (complement (coproduct R S)) = eval (with (complement R) (complement S)) := by
+apply funext; intro ab; apply funext; intro cd
+cases ab <;> cases cd
+. simp [Relation.eval]
+. simp [Relation.eval]
+. simp [Relation.eval]
+. simp [Relation.eval]
+
+
+-- theorem Relation.product_coproduct__dist (R: Relation α α) (S: Relation α α) (T: Relation α α) :
+--   eval (product (coproduct R S) T) = eval (coproduct (product R T) (product S T)) := sorry
+
+-- theorem Relation.coproduct_product_dist (R: Relation α β) (S: Relation γ δ) (T: Relation ε ζ) :
+-- eval (product (coproduct R S) T) = eval (coproduct (product R T) (product S T))  := by sorry
+
+--  Equiv.sumProdDistrib is the distributivity equivalence for Sum and Product types. We need to apply this so the types match on either side of the eqution.
+
+#print Relation.eval
+#print Relation.Pairs
+
+
+-- (R⊕S)⊗T = (R⊗T)⊕(S⊗T)
+theorem Relation.coproduct_product_dist (R: Relation α β) (S: Relation γ δ) (T: Relation ε ζ) :
+  eval (product (coproduct R S) T) =
+    fun (a:(α ⊕ γ) × ε) (b: (β ⊕ δ) × ζ) =>
+      let prodPlusProd := eval (coproduct (product R T) (product S T))
+      let isoDomain := (Equiv.sumProdDistrib α γ ε)
+      let isoCodomain := (Equiv.sumProdDistrib β δ ζ)
+      prodPlusProd (isoDomain a) (isoCodomain b) := by
+  apply funext; intro a; apply funext; intro b
+  dsimp [Relation.eval, Equiv.sumProdDistrib]
+  cases a.1 <;> cases b.1
+  . simp
+  . simp
+  . simp
+  . simp
+
+-- T⊕(R⊗S) = (T⊕R) ⊗ (T⊕S)
+theorem Relation.product_coproduct_dist (R: Relation α β) (S: Relation γ δ) (T: Relation ε ζ) :
+  eval (coproduct T (product R S)) =
+    fun (a:(ε ⊕ α × γ)) (b: ζ ⊕ β × δ) =>
+      let coprodTimesCoprod := eval (product (coproduct T R) (coproduct T S))
+
+      let isoA := (Equiv.prodSumDistrib ε α γ )
+      let isoA' := (Equiv.sumProdDistrib ε α γ )
+       -- I need:   ε ⊕ α × γ ≃ (ε ⊕ α) × (ε ⊕ γ))
+       -- Equiv.prodSumDistrib ε α γ gives: ε × (α ⊕ γ) ≃ ε × α ⊕ ε × γ
+       -- Equiv.sumProdDistrib ε α γ gives: (ε ⊕ α) × γ ≃ ε × γ ⊕ α × γ
+       -- These are just two sides of the same distributive law. But I need the other distributive law for adding over a product.
+
+
+      let isoB := (Equiv.prodSumDistrib β δ ζ)
+      coprodTimesCoprod (isoA a) (isoB b) := by
+  apply funext; intro a; apply funext; intro b
+  dsimp [Relation.eval, Equiv.sumProdDistrib]
+  cases a <;> cases b
+    . simp
+    . simp
+    . simp
+    . simp
+
+
+-- theorem Relation.product_coproduct__dist (R: Relation α β) (S: Relation γ δ) (T: Relation ε ζ) :
+--   eval (product (coproduct R S) T) = eval (coproduct (product R T) (product S T)) := sorry
+
+
+-- @[simp]
+-- theorem Relation.complement_coproduct (R: Relation α β) (S: Relation γ δ) :
+--   eval (complement (coproduct R S)) = eval (coproduct (complement R) (complement S)) := by
+--   apply funext; intro αβ ; apply funext; intro  βδ
+--   cases αβ <;> cases  βδ
+--   . simp [Relation.eval]
+--   . simp [Relation.eval, Relation.complement, Relation.coproduct]
+--   . simp [Relation.eval]
+--   . simp [Relation.eval]
+
+
+
+-- theorem Relation.complement_relativeComp (R: Relation α β) (S: Relation β γ) :
+--   eval (complement (relativeComp R S)) = eval (relativeComp (complement R) (complement S)) := by
+--   apply funext; intro a; apply funext; intro c
+--   simp [Relation.eval, Relation.complement, Relation.relativeComp]
+--   apply Iff.intro
+--   . intro h
+--     by_contra h'
+--     case h.h.mp =>
+--       cases h with
+--       | intro c₁ hc₁ =>
+--         apply h' c₁
+--         . simp [Relation.eval, Relation.complement] at hc₁
+--           exact hc₁.left
+--         . simp [Relation.eval, Relation.complement] at hc₁
+--           exact hc₁.right
+--   . intro h
+--     by_contra h'
+--     case h.h.mpr =>
+--       by_contra h'
+--       apply h' (fun x hRax => h x hRax)
